SciLean/Tactic/DataSynth/Theorems.lean
@@ -10,6 +10,116 @@ open Mathlib.Meta.FunProp
 namespace SciLean.Tactic.DataSynth
 
 
+inductive LambdaTheorem where
+  /-- Composition theorem
+
+  The theorem should have roughly the following form
+  ```
+  (g : X → Y) (f : Y → Z) (hg : P g g') (hf : P f f') → P (f∘g) fg'
+  ```
+  and `gId`, `fId`, `hgId`, `hfId` are indices of corresponding arguments in the theorem `thmName`
+   -/
+  | comp (dataSynthName thrmName : Name) (gId fId hgId hfId : Nat)
+  /-- Let binding theorem
+
+  The theorem should have roughly the following form
+  ```
+  (g : X → Y) (f : Y → X → Z) (hg : P g g') (hf : P f f') → P (fun x => let y := g x; f y x) fg'
+  ```
+  and `gId`, `fId`, `hgId`, `hfId` are indices of corresponding arguments in the theorem `thmName`
+  -/
+  | letE (dataSynthName thrmName : Name) (gId fId hgId hfId : Nat)
+  /-- Pi theorem
+
+  The theorem should have roughly the following form
+  ```
+  (f : X → I → Y) (hf : ∀ i, P (f · i) (f' i)) → P (fun x i => f x i) f'
+  ```
+  and `fId`, `hfId` are indices of corresponding arguments in the theorem `thmName`
+  -/
+  | pi   (dataSynthName thrmName : Name) (fId hfId : Nat)
+  /-- Constant theorem
+
+  The theorem should have roughly the following form
+  ```
+  (y : Y) → P (fun x => y) c'
+  `` -/
+  | const (dataSynthName thrmName : Name)
+  /-- Projection theorem
+
+  This theorem says that if we can restrict `f : X → Y` to a smaller domain `X₁` and we know how
+  to transform this restriction then we know how to transform `f`.
+
+  The theorem should have roughly the following form
+  ```
+  (f : X → Y) (g : X₁ → Y) (p₁ : X → X₁) (p₂ : X → X₂) (q : X₁ → X₂ → X) (hg : P g g') → P f f'
+  ```
+
+  TODO: There has to be some condition on p₁,p₂,q that they really form a decomposition.
+  -/
+  | proj (dataSynthName thrmName : Name) (fId gId p₁Id p₂Id qId hgId : Nat)
+  deriving Inhabited
+
+inductive LambdaTheoremType where | comp | letE | pi | const | proj
+  deriving BEq, Inhabited, Hashable
+
+/-- Get name of the theorem. -/
+def LambdaTheorem.thmName (thm : LambdaTheorem) : Name :=
+  match thm with
+  | .comp _ thmName _ _ _ _ => thmName
+  | .letE _ thmName _ _ _ _ => thmName
+  | .pi   _ thmName _ _     => thmName
+  | .const _ thmName        => thmName
+  | .proj _ thmName _ _ _ _ _ _ => thmName
+
+/-- Get name of the data synthesis. -/
+def LambdaTheorem.dataSynthName (thm : LambdaTheorem) : Name :=
+  match thm with
+  | .comp dataSynthName _ _ _ _ _ => dataSynthName
+  | .letE dataSynthName _ _ _ _ _ => dataSynthName
+  | .pi   dataSynthName _ _ _     => dataSynthName
+  | .const dataSynthName _        => dataSynthName
+  | .proj dataSynthName _ _ _ _ _ _ _ => dataSynthName
+
+/-- Get proof of a theorem. -/
+def LambdaTheorem.getProof (thm : LambdaTheorem) : MetaM Expr :=
+  match thm with
+  | .comp _ thmName _ _ _ _ => mkConstWithFreshMVarLevels thmName
+  | .letE _ thmName _ _ _ _ => mkConstWithFreshMVarLevels thmName
+  | .pi   _ thmName _ _     => mkConstWithFreshMVarLevels thmName
+  | .const _ thmName        => mkConstWithFreshMVarLevels thmName
+  | .proj _ thmName _ _ _ _ _ _ => mkConstWithFreshMVarLevels thmName
+
+/-- Get type of the theorem. -/
+def LambdaTheorem.type (thm : LambdaTheorem) : LambdaTheoremType :=
+  match thm with
+  | .comp .. => LambdaTheoremType.comp
+  | .letE .. => LambdaTheoremType.letE
+  | .pi   .. => LambdaTheoremType.pi
+  | .const .. => LambdaTheoremType.const
+  | .proj .. => LambdaTheoremType.proj
+
+/-- Enviroment extension for lambda theorems -/
+initialize lambdaTheoremsExt : SimpleScopedEnvExtension LambdaTheorem (Std.HashMap (Name×LambdaTheoremType) (Array LambdaTheorem)) ←
+  registerSimpleScopedEnvExtension {
+    name     := by exact decl_name%
+    initial  := {}
+    addEntry := fun d e => d.alter (e.dataSynthName,e.type)
+      (fun v? => match v? with | .some v => v.push e | .none => #[e])
+  }
+
+/-- Add lambda theorem to the enviroment. -/
+def addLambdaTheorem (thm : LambdaTheorem) : CoreM Unit :=
+  lambdaTheoremsExt.add thm
+
+/-- Add lambda theorem to the enviroment. -/
+def getLambdaTheorems (dataSynthName : Name) (thmType : LambdaTheoremType) :
+    CoreM (Array LambdaTheorem) := do
+  return (lambdaTheoremsExt.getState (← getEnv))[(dataSynthName,thmType)]?.getD #[]
+
+
+----------------------------------------------------------------------------------------------------
+
 /-- Generalized transformation theorem -/
 structure DataSynthTheorem where
   /-- Name of generalized transformation -/
