SciLean/Analysis/AdjointSpace/DefHasAdjoint.lean
@@ -1,0 +1,164 @@
+import SciLean.Analysis.AdjointSpace.HasAdjoint
+-- import SciLean.Tactic.DataSynth.ArrayOperations
+import SciLean.Tactic.DataSynth.Elab
+import SciLean.Tactic.LSimp
+
+namespace Scilean.Tactic.DataSynth.HasAdjoint
+
+open SciLean
+
+open Lean Elab Command Meta Qq
+
+def getScalar? : MetaM (Option (Expr×Expr)) := do
+  (← getLCtx).findDeclRevM? fun decl => do
+    let type ← whnf decl.type
+    dbg_trace (← ppExpr type)
+    if (type.isAppOfArity ``RealScalar 1) ||
+       (type.isAppOfArity ``RCLike 1) ||
+       (type.isAppOfArity ``Scalar 2)  then
+      return (decl.toExpr, decl.type.appArg!)
+    else
+      return none
+
+def fixTypeUniverseQ (X : Expr) : MetaM ((u : Level) × Q(Type $u)) := do
+  let .sort (Level.succ u) ← whnf (← inferType X) | throwError "not a type{indentExpr X}, has type {← ppExpr (← inferType X )}"
+  return ⟨u,X⟩
+
+def getScalarQ? : MetaM (Option ((u : Level) × (R : Q(Type u)) × Q(RCLike $R))) := do
+  (← getLCtx).findDeclRevM? fun decl => do
+    let type ← whnf decl.type
+    if (type.isAppOfArity ``RealScalar 1) ||
+       (type.isAppOfArity ``RCLike 1) ||
+       (type.isAppOfArity ``Scalar 2) then
+      let R := type.appArg!
+      let ⟨u,R⟩ ← fixTypeUniverseQ R
+      let inst ← synthInstanceQ q(RCLike $R)
+      return some ⟨u,R,inst⟩
+    else
+      return none
+
+
+/-- For function `f` return `HasRevFDerivUpdate` statement in specified arguments `args`.
+
+The result `(e,n,lvls)` is an expression `e` of the statement where the first `n` arguments are
+considered as inputs and rest as output. `lvls` is list of universe parameter names.
+-/
+def getSimpleGoal (fId : Name) (argNames : Array Name)
+    (extra : TSyntaxArray `Lean.Parser.Term.bracketedBinder) :
+    TermElabM (Expr × ℕ × List Name) := do
+
+  let info ← getConstInfo fId
+
+  forallTelescope info.type fun xs _ => do
+  Term.elabBinders extra.raw fun extraArgs => do
+
+    -- split arguments `xs` into main and other
+    let (mainArgs, otherArgs) ← xs.splitM (fun x => do
+      let n ← x.fvarId!.getUserName
+      return argNames.contains n)
+
+    -- check if all arguments are present
+    for argName in argNames do
+      if ← mainArgs.allM (fun a => do pure ((← a.fvarId!.getUserName) != argName)) then
+        throwError s!"function `{fId}` does not have argument `{argName}`"
+
+    -- find scalar field and its instance
+    let some ⟨_,R,_⟩ ← getScalarQ?
+      | throwError "can't determinal scalar field"
+
+    let lvlNames := info.levelParams
+    let lvls := lvlNames.map (fun p => Level.param p)
+    let f ← liftM <|
+      mkLambdaFVars mainArgs (mkAppN (Expr.const info.name lvls) xs)
+      >>=
+      mkUncurryFun' mainArgs.size
+
+    let goal ← mkAppM ``HasAdjoint #[R,f]
+    -- eta expand rest of the arguments
+    let goal ← forallTelescope (← inferType goal) fun ys _ =>
+      mkForallFVars ys (goal.beta ys)
+
+    let args := otherArgs++extraArgs
+    let statement ← mkForallFVars args goal
+
+    let fvars := (Lean.collectFVars {} statement).fvarIds
+    if h : fvars.size ≠ 0 then
+      throwError m!"resulting statement contains free variable {Expr.fvar fvars[0]}\n{statement}"
+
+    let mvars := statement.collectMVars {} |>.result
+    if h : mvars.size ≠ 0 then
+      throwError m!"resulting statement contains meta variable {Expr.mvar mvars[0]}\n{statement}"
+
+    return (statement,args.size,lvlNames)
+
+
+open Qq in
+elab "def_has_adjoint" fId:ident "in" args:ident* bs:bracketedBinder* "by" tac:tacticSeq : command => do
+
+  Elab.Command.liftTermElabM <| do
+  -- resolve function name
+  let fId ← ensureNonAmbiguous fId (← resolveGlobalConst fId)
+  let argNames := args.map (fun id => id.getId)
+
+  let (simpleGoal,n,lvls) ← getSimpleGoal fId argNames bs
+  -- let (compGoal,m,lvls') ← getCompositionalGoal fId argNames bs
+
+  forallBoundedTelescope simpleGoal n fun xs e => do
+    let (_,_,statement) ← forallMetaTelescope (← etaExpand e)
+
+    let proof ← mkFreshExprMVar statement
+    let (_,_) ← runTactic proof.mvarId! tac
+
+    let suffix := (argNames.foldl (init:=`arg_) (·.appendAfter ·.toString))
+    let thmName := fId.append suffix |>.append `HasAdjoint_simple_rule
+
+    -- let statement' := ← instantiateMVars (← mkForallFVars xs statement)
+
+    -- -- let fvars := (Lean.collectFVars {} statement').fvarIds
+    -- -- if h : fvars.size ≠ 0 then
+    -- --   throwError m!"resulting statement contains free variable {Expr.fvar fvars[0]}\n{statement}"
+
+    -- -- let mvars := statement'.collectMVars {} |>.result
+    -- -- if h : mvars.size ≠ 0 then
+    -- --   throwError m!"resulting statement contains meta variable {Expr.mvar mvars[0]}\n{statement}"
+
+    -- let proof' := ← instantiateMVars (← mkLambdaFVars xs proof)
+
+    -- IO.println s!"{← ppExpr statement'}"
+    -- IO.println s!"{← ppExpr (← inferType proof')}"
+
+    -- let fvars := (Lean.collectFVars {} proof').fvarIds
+    -- if h : fvars.size ≠ 0 then
+    --   throwError m!"resulting statement contains free variable {Expr.fvar fvars[0]}\n{statement}"
+
+    -- let mvars := proof'.collectMVars {} |>.result
+    -- if h : mvars.size ≠ 0 then
+    --   throwError m!"resulting statement contains meta variable {Expr.mvar mvars[0]}\n{statement}"
+
+    -- if statement'.hasMVar then
+    --   throwError m!"proof has mvar"
+
+    -- if proof'.hasMVar then
+    --   throwError m!"statement has mvar"
+
+    let thmVal : TheoremVal :=
+    {
+      name  := thmName
+      type  := ← instantiateMVars (← mkForallFVars xs statement)
+      value := ← instantiateMVars (← mkLambdaFVars xs proof)
+      levelParams := lvls
+    }
+
+    addDecl (.thmDecl thmVal)
+    Tactic.DataSynth.addTheorem thmName
+
+
+variable {R} [RealScalar R] {X} [NormedAddCommGroup X] [AdjointSpace R X]
+
+def foo (x y : X) :=
+  let z := (3:R)•x + x
+  x + (2:R)•(y + (4:R)•z)
+
+def_has_adjoint foo in x y by
+  unfold foo
+  data_synth => dsimp -zeta
