SciLean/Tactic/DataSynth/HasRevFDerivUpdate.lean
@@ -129,6 +129,17 @@ theorem proj_rule (f : X → Y) {g'}
         let dx₁ := dg dy dx₁
         q dx₁ dx₂)) := by sorry_proof
 
+open Lean Meta
+#eval show MetaM Unit from do
+   Tactic.DataSynth.addLambdaTheorem (.const ``HasRevFDerivUpdate ``const_rule )
+   Tactic.DataSynth.addLambdaTheorem (.comp ``HasRevFDerivUpdate ``comp_rule
+      (← getConstArgId ``comp_rule `g) (← getConstArgId ``comp_rule `f) (← getConstArgId ``comp_rule `hg) (← getConstArgId ``comp_rule `hf))
+   Tactic.DataSynth.addLambdaTheorem (.letE ``HasRevFDerivUpdate ``let_rule
+      (← getConstArgId ``let_rule `g) (← getConstArgId ``let_rule `f) (← getConstArgId ``let_rule `hg) (← getConstArgId ``let_rule `hf))
+   Tactic.DataSynth.addLambdaTheorem (.pi ``HasRevFDerivUpdate ``pi_rule (← getConstArgId ``pi_rule `f) (← getConstArgId ``pi_rule `hf))
+   Tactic.DataSynth.addLambdaTheorem (.proj ``HasRevFDerivUpdate ``proj_rule
+      (← getConstArgId ``proj_rule `f) (← getConstArgId ``proj_rule `g) (← getConstArgId ``proj_rule `p₁) (← getConstArgId ``proj_rule `p₂) (← getConstArgId ``proj_rule `q) (← getConstArgId ``proj_rule `hg))
+
 
 end HasRevFDerivUpdate
 
